updating to 8.12.2

theories/Demo.v
@@ -5,7 +5,7 @@ Locate Point.
 (* a small example *)
 
 Lemma ex1 : forall A B C D:Point,
-    rk(A::B::C::nil) = 3 ->
+    rk(A::B::D::nil) = 3 ->
     rk(A::C::D::nil) = 2 ->
     rk(A::C::nil) = 2 ->
     rk(C::D::nil) = 2 ->
@@ -14,22 +14,54 @@ Proof.
   intros.
   (* call the prover *)
   pprove.
-Admitted.
-
-Lemma ex1_solved : forall A B C D:Point,
-    rk(A::B::C::nil) = 3 ->
-    rk(A::C::D::nil) = 2 ->
-    rk(A::C::nil) = 2 ->
-    rk(C::D::nil) = 2 ->
-    rk(A::B::C::nil) = 3.
-Proof.
-intros P1 P2 P3 P4 
-HP1P3eq HP1P2P3eq HP3P4eq HP1P3P4eq .
-
-assert(HP1P2P3M : rk(P1 :: P2 :: P3 ::  nil) <= 3) by (solve_hyps_max HP1P2P3eq HP1P2P3M3).
-assert(HP1P2P3m : rk(P1 :: P2 :: P3 ::  nil) >= 1) by (solve_hyps_min HP1P2P3eq HP1P2P3m1).
-intuition.
+  Require Import pprove_ex1.
+  eauto with ranks.
 Qed.
+Check ex1.
 
-Check ex1_solved.
-Print ex1_solved.
+
+Definition triple (X Y Z : Point) : (list Point) := (X :: Y :: Z :: nil).
+
+Lemma desargues : forall a b c A B C alpha beta gamma O : Point,
+
+forall raAO : rk(triple a A O)=2, 
+forall rbBO : rk(triple b B O)=2, 
+forall rcCO : rk(triple c C O)=2, 
+forall rABC : rk(triple A B C)=3, 
+forall rabc : rk(triple a b c)=3, 
+
+forall rABCabc : rk(A::B::C::a::b::c::nil)=4, 
+
+forall rABgamma : rk(triple A B gamma)=2,
+forall rabgamma : rk(triple a b gamma)=2,
+
+forall rACbeta : rk(triple A C beta)=2,
+forall racbeta : rk(triple a c beta)=2,
+
+forall rBCalpha : rk(triple B C alpha)=2,
+forall rbcalpha : rk(triple b c alpha)=2,
+
+
+
+forall raA : rk(a:: A :: nil)=2,
+forall rcC : rk(c:: C :: nil)=2,
+forall rbB : rk(b:: B:: nil)=2,
+(*  rk(a::b::c::nil)=3 ->
+  rk(A::B::C::nil)=3 ->*)
+  
+  rk(O::a::nil)=2->
+  rk(O::b::nil)=2->
+  rk(O::c::nil)=2->
+  rk(O::A::nil)=2->
+  rk(O::B::nil)=2->
+  rk(O::C::nil)=2->
+  
+  rk ( alpha ::beta ::gamma::nil) = 2.
+Proof.
+  unfold triple.
+  intros.
+  pprove.
+  Require Import pprove_desargues. 
+  eauto with ranks.
+Qed.
+  
